Pdl/Interpolation/Theorem.lean
@@ -2,7 +2,6 @@ import Mathlib.Data.Finset.Basic
 
 import Pdl.Interpolation.Def
 import Pdl.Completeness.Theorem
-import Pdl.UniCompleteness.UniTheorem
 
 /-! # Interpolation (Section 7) -/
 
@@ -22,7 +21,7 @@ theorem interpolation {φ ψ : Formula} :
     rw [← consIffSat _ (by simp)] at hyp -- using completeness
     simp [consistent,inconsistent] at hyp
     rcases hyp with ⟨tab⟩
-    have := UniGame.Tableau.toUniformViaGame (by simp) tab -- Yeah.
+    have := Tableau.toUniformViaGame (by simp) tab -- Yeah.
     rcases this with ⟨t, t_h⟩
     exact ⟨t, t_h⟩
   rcases have_tab with ⟨tab, tab_uni⟩
